\documentclass{article}
\begin{document}
\noindent\textbf{ADD-BITS(A, B)}\\
\indent n = MAX(A.length, B.length) + 1\\
\indent C = ARRAY(INTEGER, n)\\
\indent carry = 0\\
\indent i = C.length\\
\indent j = A.length\\
\indent k = B.length\\
\indent while i <= n\\
\indent\indent if j > 0 and k > 0\\
\indent\indent\indent C[i] = (A[j] + B[k] + carry) mod 2 + carry\\
\indent\indent\indent carry = (A[j] + B[k] + carry) / 2\\
\indent\indent else if j == 0 and k == 0\\
\indent\indent\indent C[i] = carry\\
\indent\indent else if j = 0\\
\indent\indent\indent C[i] = (B[k] + carry) mod 2\\
\indent\indent\indent carry = (B[k] + carry)  / 2\\
\indent\indent else\\
\indent\indent\indent C[i] = (A[j] + carry) mod 2\\
\indent\indent\indent carry = (A[j] + carry)  / 2\\
\indent\indent if j == 0\\
\indent\indent\indent j = j - 1\\
\indent\indent if k == 0\\
\indent\indent\indent k = k - 1\\
\indent\indent i = i - 1\\\\

\noindent \textbf{Loop invariant:} at the start of every
iteration, C[i-1 .. n] will always have the sum of bits of
A[j-1 .. A.length] and B[k-1 .. B.length]\\

\noindent \textbf{Initialization:} C[ n-1 .. n] is the null array,
therefore it contains the sum of A[A.length-1, A.length]=null
and B[B.length-1 .. B.length]=null\\
\noindent \textbf{Maintenance:} Suppose C[i .. n] contains the sum
of B[k .. B.length] and \\A[j-1 .. A.length] and the carry, 
if j and k are still greater than the lower bounds of both A and B
then C[i] = (B[k] + A[j] + carry) mod 2, which means that C[i]
will hold the sum of the tow plus whatever carry out there from
the previous operation. If we already summed either of all 
elements of A, or B or both, C[i] will take the carry, as 
if A[j] or B[k] or both of them are zero.\\
Therefore C[i] will hold the result of the sum of A[j] and B[k]
plus the carry. \\Therefore C[i-1 .. n] will contain the sum of
B[k-1 .. B.length] and \\A[j-1 .. A.length] and the  carry\\
\noindent \textbf{Termination:} On termination we
have i = 0, k = 0, j = 0 , therefore C[1 .. n] contains the sum of
B[1 .. B.length] and A[ 1 .. A.length].\\
\end{document}
