\documentclass{article}
\usepackage{amsmath}
\begin{document}
\begin{equation}
T(n) =
\begin{cases}
2 &if \ n = 2 \\
2T(\frac{n}{2}) \ + n & if n = 2^k, \ for \ k > 1
\end{cases}
\end{equation}
\begin{align*}
T(n) = 2T(\frac{n}{2}) + n \\
and\\
T(\frac{n}{2}) = 2T(\frac{n}{4}) + \frac{n}{2}
&\Rightarrow T(n) = 4T(\frac{n}{4}) + 2n \\
Knowing\\
T(n/4) = 2T(\frac{n}{8}) + \frac{n}{4}
&\Rightarrow T(n) = 8T(\frac{n}{8}) + 3n \\
\ldots\\
&\Rightarrow T(n) = 2^i T(\frac{n}{2^i}) + in\\
We \ have:\\
T(n/2^i) = 2  & \Leftrightarrow \frac{n}{2^i} = 2 \\
\frac{n}{2^i} = 2   & \Leftrightarrow i + 1 = \frac{lg_2(n)}{lg_2(2)}\\
Therfore\\
T(n) = 2^{lg_2(n)}  + (lg_2(n) - 1) n  &
\Leftrightarrow T(n) = n (1 - 1 + lg_2(n)) \\
& \Leftrightarrow T(n) = nlg_2(n)
\end{align*}
\end{document}
